---
tags:
  - m
  - 3te_Klasse
---
```math
||{"id":1495987931}||

f(x)=\frac{3x+x²}{x-1}
u'(x)=3+2x
v'(x)=1
f'(x)=(3+2x)*(x-1)-\frac{(1)*(3x+x²)}{(x-1)²}=\frac{(3+2x)*(x-1)-3-x²}{(x-1)²}
```
3.50)
a)
```math
||{"id":1686509877931}||

f(x)=\frac{x²+1}{x}
f'(x)=\frac{2x*x-1*(x²+1)}{x²}=\frac{2x²-x²-1}{x²}=\frac{x²-1}{x²}
```
b)
```math
||{"id":473356564098}||

f(x)=(\frac{1}{x²+1})
f'(x)=\frac{0*(x²+1)-2x*1}{(x²+1)²}=-\frac{2x}{(x²+1)²}
```
d)
```math
||{"id":1000157281422}||

f(x)=\frac{x}{e^x}
f'(x)=\frac{e^x*(1-x)}{e^x}=\frac{1-x}{e^x}
```
e)
```math
||{"id":1114203845978}||

f(x)=\frac{1}{\sin(x)}
f'(x)=\frac{0*\sin(x)-\cos(x)}{(\sin(x))²}=\frac{\cos(x)}{(\sin(x))²}
```
