---
tags:
  - m
  - 3te_Klasse
---
3.28a)
```math
||{"id":1609097473726}||

f(x)=2x²+2x+1
f'(x)=4x¹+2
```
c)
```math
||{"id":50981288364}||

f(x)=\frac{3}{x²}-\frac{4}{x}=3x^{-2}-4x^{-1}
f'(x)=-6x^{-3}+4x^{-2}=-\frac{6}{x³}+\frac{4}{x²}
```
f)
```math
||{"id":249053329159}||

f(x)=\frac{x²+1}{2x}=\frac{x²}{2x}+\frac{1}{2x}=\frac{x}{2}+\frac{x^{-1}}{2}
f'(x)=\frac{1}{2}-\frac{1x^{-2}}{2}=-\frac{1}{2x²}+\frac{1}{2}
```
3.26)
a)
```math
||{"id":1454345359785}||

f(x)=2x²
f'(x)=2*2x^{2-1}=4x
```
b)
```math
||{"id":877527017994}||

f(x)=\frac{x}{2}
f'(x)=\frac{1*x^{1-1}}{2}=\frac{1*x^{0}}{2}=\frac{1}{2}
```

c)
```math
||{"id":970221368795}||

f(x)=2x^{-1}
f'(x)=-1*2x^{-1-1}=-1*2x^{-2}=-2x^{-2}=\frac{.2}{x²}
```
d)
```math
||{"id":757498232671}||

f(x)=\frac{1}{3x}=\frac{x^{-1}}{3}
f'(x)=\frac{-1x^{-2}}{3}=-\frac{1}{3x²}
```
e)
```math
||{"id":1352343433582}||

f(x)=\frac{1}{x²}=x^{-2}
f'(x)=-2x^{-3}=\frac{2}{x³}
```
f)
```math
||{"id":164478647853}||

f(x)=\frac{1}{4x³}=\frac{x^{-3}}{4}
f'(x)=\frac{3}{4}*x^{-4}=-\frac{3}{4x⁴} 
```
g)
```math
||{"id":146415033688}||

f(x)=(3x)²=9x²
f'(x)=18x
```
h)
```math
||{"id":1209908531270}||

f(x)=\sqrt[3]{ x }=x^{\frac{1}{3}}
f'(x)=\frac{1}{3}*x^{-\frac{2}{1}}=\frac{1}{3*\sqrt[3]{x²}}
```
i)
```math
||{"id":1062332842432}||

f(x)=x*\sqrt{ x }=x^{\frac{2}{2}}
f'(x)=\frac{3}{2}*x^{1/2-2/2}=\frac{3}{2}\sqrt{ x }
```
j)
```math
||{"id":104414381423}||

f(x)=\sqrt{ 2x }=\sqrt{ 2 }*x^{\frac{1}{2}}
f'(x)=\frac{\sqrt{ 2 }}{2*\sqrt{ x }}=\frac{\sqrt{ 2 }}{\sqrt{ 2²x }}=\sqrt{ \frac{2}{2²\times} }=\sqrt{ \frac{1}{2x} }=\frac{1}{\sqrt{ 2x }}
```
3.32)a)
```math
||{"id":1424555366248}||

y=2x²-12x+21
y'=4x-12
0=4x-12 
12=4x
x=3
2*3²-12*3+21=3
S(3|3)
```
3.35)
```math
||{"id":295119000421}||

y=ax²+bx+c
y'=2ax+b
x=3, Steigung 0.5⇒f'(3)=0.5⇒2*a*3+b=0.5
```
P(1|3),x=0⇒y-Achse geschnitten
```math
||{"id":734708710342}||

f(1)=0
0=a*1²+b*1+c

```
P(0|3),x=0⇒y-Achse geschnitten
```math
||{"id":1532632945501}||

3=a*0+b*0+c⇒c=3
```
```math
||{"id":289643842388}||

|:-0.5=6a+b|-
||:0=a+b+3|
-0.5=5a-3
2.5=5a
a=\frac{1}{2}
0=\frac{1}{2}+b+3
b=- \frac{7}{2}
⇒y=\frac{1}{2}x²-\frac{7}{2}x+3
```
3.42)
a)
```math
||{"id":839691508885}||

s(t)=v_{0}t+\frac{1}{2}a*t²
s'(t)=v(t)
v'(t)=a(t)
s'(t)=v(t)=v_{0}+a*t
```
b)
```math
||{"id":1385642251437}||

v_{0}=45kmh
a=4 \frac{m}{s²}
v(3)=\frac{45}{3.6}+4*3=24 m/s=88,2 kmh
```
3.28)
b)
```math
||{"id":1181985723778}||

f(x)=x+x^{-1}
f'(x)=1-1*x^{-2}=1-x^{-2}=1-\frac{1}{x^{-2}}
```
d)
```math
||{"id":658600491113}||

f(x)=\frac{x+1}{2}=\frac{x}{2}+\frac{1}{2}
f'(x)=\frac{1}{2}
```

e)
```math
||{"id":1655073174483}||

f(x)=\frac{x+1}{x}=\frac{x}{x}+\frac{1}{x}=1+1x^{-1}
f'(x)=-x^{-2}=- \frac{1}{x²}
```
3.29)
a)
```math
||{"id":1265166888200}||

f(x)=-\cos x+3*\tan x
f'(x)=\sin x+\frac{3}{\cos²x}
```
e)
```math
||{"id":153521589843}||

f(x)=\ln x+\ln_{2}
f'(x)=\frac{1}{x}
```
b)
```math
||{"id":112495509974}||

f(x)=\frac{\sin x }{2*\cos x}=\frac{1}{2}*\tan x
f'(x)=\frac{1}{2*\cos²x}
```
c)
```math
||{"id":83297599398}||

f(x)=\frac{x}{2}+e^x
f'(x)=\frac{1}{2}+e^x
```
d)
```math
||{"id":526844798184}||

f(x)=\frac{3x²-2^x}{2}=\frac{3}{2}*x²-\frac{1}{2}*2^x
f'(x)=3x-\frac{2^x*\ln 2}{2}
```
f)
```math
||{"id":876959150763}||

f(x)=x+3 lg x
f'(x)=\frac{1}{2}+e^x
```
