---
tags:
  - m
  - 4te_Klasse
---
1)
$$s''(t)-t+1=0$$
$$s'(t)=0$$
$$s(t)=0$$
$$t=1$$

$$s''(t)=t-1$$
$$s'(t)= \frac{t^2}{2}+C_{1}$$
bedingung einsetzen für C1
$0= \frac{1}{2}+1+C_{1}= \frac{1}{2}$$
nochmal das von oben integrieren um auf das zu kommen
$$s(t)=\frac{t^3}{6}- \frac{t^2}{2}+ \frac{t}{2}+C_{2}$$
bedingung einsetzen für C2
$$\frac{1}{6}- \frac{1}{2}+ \frac{1}{2}+C_{2}= - \frac{1}{6}$$
$$s(t)=\frac{t^3}{6}- \frac{t^2}{2}+ \frac{t}{2}- \frac{1}{6}$$
2)
$$y'=-4xy$$
$$\frac{dy}{dx}= -4 xy | * dy :y$$
$$\frac{1}{y}dy= -4xdx$$
intgrieren
$$\ln(y)$$
something